
This is a logical formula.
((p → q) ∧ (q → r)) → (p → r)


This is a proof tree in overleaf friendly latex:
Proof for $\neg (p \mor q) \impl (\neg p \mand \neg q)$:
\begin{prooftree}
% Left branch
\AxiomC{~}
\ax
\UnaryInfC{$p \fCenter p, \, q $}
\rlabel{\neg}
\UnaryInfC{$\fCenter p, \, q,\, \neg p$}
% Right branch
\AxiomC{~}
\ax
\UnaryInfC{$q \fCenter p, \, q $}
\rlabel{\neg}
\UnaryInfC{$\fCenter p, \, q,\, \neg q$}
% BinaryInfC creates two branches
\rlabel{\mand}
\BinaryInfC{$\fCenter p, \, q,\, \neg p \mand \neg q$}
\rlabel{\mor}
\UnaryInfC{$\fCenter p \mor q,\, \neg p \mand \neg q$}
\llabel{\neg}
\UnaryInfC{$\neg (p \mor q) \fCenter \neg p \mand \neg q$}
\rlabel{\impl}
\UnaryInfC{$\fCenter \neg (p \mor q) \impl (\neg p \mand \neg q)$}
\end{prooftree}

old notes:

\begin{prooftree}
% AxiomC completes the proof tree.
\AxiomC{~}
\ax
\UnaryInfC{$p,\, q \fCenter p$}
\rlabel{\impl}
\UnaryInfC{$p \fCenter (q \impl p)$}
\rlabel{\impl}
% UnaryInfC creates a branch
\UnaryInfC{$\fCenter p \impl (q \impl p)$}
\end{prooftree}

Proof for $\neg (p \mor q) \impl (\neg p \mand \neg q)$:
\begin{prooftree}
% Left branch
\AxiomC{~}
\ax
\UnaryInfC{$p \fCenter p, \, q $}
\rlabel{\neg}
\UnaryInfC{$\fCenter p, \, q,\, \neg p$}
% Right branch
\AxiomC{~}
\ax
\UnaryInfC{$q \fCenter p, \, q $}
\rlabel{\neg}
\UnaryInfC{$\fCenter p, \, q,\, \neg q$}
% BinaryInfC creates two branches
\rlabel{\mand}
\BinaryInfC{$\fCenter p, \, q,\, \neg p \mand \neg q$}
\rlabel{\mor}
\UnaryInfC{$\fCenter p \mor q,\, \neg p \mand \neg q$}
\llabel{\neg}
\UnaryInfC{$\neg (p \mor q) \fCenter \neg p \mand \neg q$}
\rlabel{\impl}
\UnaryInfC{$\fCenter \neg (p \mor q) \impl (\neg p \mand \neg q)$}
\end{prooftree}

\bigskip

Derivation with an open branch:
\begin{prooftree}
  \AxiomC{$p \fCenter q$}

  \AxiomC{~}
  \ax
  \UnaryInfC{$p \fCenter p$}

  \rlabel{\mand}
  \BinaryInfC{$ p \fCenter q \mand p$ }
  \rlabel{\impl}
  \UnaryInfC{$\fCenter p \impl (q \mand p)$ }
\end{prooftree}

\bigskip


\noindent It's also possible to create inline proofs - this can be useful when defining or referencing rules.
\\
As an example, here is the $\mand$-right rule:
\AxiomC{$\Gamma \fCenter A ,\, \Delta$}
\AxiomC{$\Gamma \fCenter B ,\, \Delta$}
\rlabel{\mand}
\BinaryInfC{$\Gamma \fCenter A \mand B, \, \Delta$}
\DisplayProof

\end{document}



Proof for $\forall x \exists y ( p(x) \land (p(y) \rightarrow q(x)) ) \rightarrow \forall z q(z)$:
\begin{prooftree}
% Left branch
\AxiomC{~}
\ax
\UnaryInfC{$\forall x \exists y ( p(x) \land (p(y) \rightarrow q(x)) ) \fCenter \forall x \exists y ( p(x) \land (p(y) \rightarrow q(x)) )$}
\rlabel{\forall x}
\UnaryInfC{$\exists y ( p(x) \land (p(y) \rightarrow q(x)) ) \fCenter \forall x \exists y ( p(x) \land (p(y) \rightarrow q(x)) )$}
\rlabel{\exists y}
\UnaryInfC{$p(x) \land (p(y) \rightarrow q(x)) \fCenter \forall x \exists y ( p(x) \land (p(y) \rightarrow q(x)) )$}
\rlabel{\land}
\UnaryInfC{$p(x) \fCenter \forall x \exists y ( p(x) \land (p(y) \rightarrow q(x)) )$}
\rlabel{\forall z}
\UnaryInfC{$\forall z q(z) \fCenter \forall x \exists y ( p(x) \land (p(y) \rightarrow q(x)) )$}
\rlabel{\rightarrow}
\UnaryInfC{$\forall x \exists y ( p(x) \land (p(y) \rightarrow q(x)) ) \rightarrow \forall z q(z) \fCenter \forall x \exists y ( p(x) \land (p(y) \rightarrow q(x)) )$}
\end{prooftree}


Proof for $((p \rightarrow r) \land (q \rightarrow r)) \rightarrow (p \rightarrow q)$:
\begin{prooftree}
  % Left branch
  \AxiomC{}
  \UnaryInfC{$p \rightarrow r \fCenter p \rightarrow r$}
  \RightLabel{$\land$}
  \UnaryInfC{$(p \rightarrow r) \land (q \rightarrow r) \fCenter (p \rightarrow r) \land (q \rightarrow r)$}
  % Right branch
  \AxiomC{}
  \UnaryInfC{$q \rightarrow r \fCenter q \rightarrow r$}
  \RightLabel{$\land$}
  \UnaryInfC{$(p \rightarrow r) \land (q \rightarrow r) \fCenter (p \rightarrow r) \land (q \rightarrow r)$}
  % Combining branches
  \RightLabel{$\rightarrow$}
  \BinaryInfC{$(p \rightarrow r) \land (q \rightarrow r) \fCenter p \rightarrow q$}
  \RightLabel{$\rightarrow$}
  \UnaryInfC{$((p \rightarrow r) \land (q \rightarrow r)) \rightarrow (p \rightarrow q) \fCenter ((p \rightarrow r) \land (q \rightarrow r)) \rightarrow (p \rightarrow q)$}
\end{prooftree}



\begin{document}

\maketitle

\section{Introduction}

This is my attempt at "Oblig 1".

\subsection{Exercise 01.1 a) f1}

Here is the solution for Exercise 01.1 a) f1:

\begin{prooftree}
% Left branch
\AxiomC{~}
\ax
\UnaryInfC{$p \fCenter p, \, q $}
\rlabel{\neg}
\UnaryInfC{$\fCenter p, \, q,\, \neg p$}
% Right branch
\AxiomC{~}
\ax
\UnaryInfC{$q \fCenter p, \, q $}
\rlabel{\neg}
\UnaryInfC{$\fCenter p, \, q,\, \neg q$}
% BinaryInfC creates two branches
\rlabel{\mand}
\BinaryInfC{$\fCenter p, \, q,\, \neg p \mand \neg q$}
\rlabel{\mor}
\UnaryInfC{$\fCenter p \mor q,\, \neg p \mand \neg q$}
\llabel{\neg}
\UnaryInfC{$\neg (p \mor q) \fCenter \neg p \mand \neg q$}
\rlabel{\impl}
\UnaryInfC{$\fCenter \neg (p \mor q) \impl (\neg p \mand \neg q)$}
\end{prooftree}

\subsection{Exercise 01.1 b) f2}

Here is the solution for Exercise 01.1 b) f2:


\AxiomC{$\Gamma \fCenter A ,\, \Delta$}
\AxiomC{$\Gamma \fCenter B ,\, \Delta$}
\rlabel{\mand}
\BinaryInfC{$\Gamma \fCenter A \mand B, \, \Delta$}
\DisplayProof

